bugs/exp.fst
@@ -1,0 +1,46 @@
+module Expressions
+
+type binop =
+| Plus
+| Minus
+| Times
+
+type id = nat
+
+type aexp =
+| AInt : int -> aexp
+| AVar : id -> aexp 
+| AOp  : binop -> aexp -> aexp -> aexp 
+
+type bexp =
+| BTrue  : bexp
+| BFalse : bexp
+| BEq    : aexp -> aexp -> bexp
+| BLe    : aexp -> aexp -> bexp
+| BNot   : bexp -> bexp
+| BAnd   : bexp -> bexp -> bexp
+
+type heap = id -> Tot int
+
+val eval_aexp : heap -> aexp -> Tot int
+let rec eval_aexp h e =
+  match e with 
+  | AInt i -> i
+  | AVar x -> h x
+  | AOp op op1 op2 ->
+     let i1 = eval_aexp h op1 in
+     let i2 = eval_aexp h op2 in
+     (match op with
+      | Plus  -> i1 + i2
+      | Minus -> i1 - i2
+      | Times -> i1 * i2)
+
+val eval_bexp : heap -> bexp -> Tot bool
+let rec eval_bexp h be =
+  match be with 
+  | BTrue -> true
+  | BFalse -> false
+  | BEq e1 e2 -> eval_aexp h e1  = eval_aexp h e2
+  | BLe e1 e2 -> eval_aexp h e1 <= eval_aexp h e2
+  | BNot be' -> not (eval_bexp h be')
+  | BAnd be1 be2 -> eval_bexp h be1 && eval_bexp h be2
